%%this document was generated by the STUPS Toolbox 2.0
\documentclass{article}
\usepackage{amssymb}
\usepackage{amsmath,amsthm}
\usepackage[ngerman,english]{babel}

\begin{document}

\section{remove lambda-rules}
\begin{description}
	\item[Before] \hfill \\ 
	$G=\left(\{	1, 0, \epsilon\},\;\{ S, A, B, D, E, C\},\;S,\;P\right)$ with
	\begin{align*}
		P=\{	S &\rightarrow ABD, \\ 
		A &\rightarrow ED\;|\;BB, \\ 
		B &\rightarrow \epsilon\;|\;AC, \\ 
		D &\rightarrow 0, \\ 
		E &\rightarrow 1, \\ 
		C &\rightarrow \epsilon\}
	\end{align*}
	\item[Step 1] nullable = \{C, A, B\}
	\item[Step 2]
	$G=\left(\{	\epsilon, 1, 0\},\;\{ S, B, D, A, E, C\},\;S,\;P\right)$ with
	\begin{align*}
		P=\{	S &\rightarrow BD\;|\;D\;|\;ABD\;|\;AD, \\ 
		B &\rightarrow A\;|\;C\;|\;\epsilon\;|\;AC, \\ 
		D &\rightarrow 0, \\ 
		A &\rightarrow ED\;|\;BB\;|\;B\;|\;\epsilon, \\ 
		E &\rightarrow 1, \\ 
		C &\rightarrow \epsilon\}
	\end{align*}
	\item[Step 3] All lambda-rules are removed and all nonterminals, that do not appear on any right side. \\ 
	$G=\left(\{	1, 0\},\;\{ S, B, D, A, E\},\;S,\;P\right)$ with
	\begin{align*}
		P=\{	S &\rightarrow BD\;|\;D\;|\;ABD\;|\;AD, \\ 
		B &\rightarrow A, \\ 
		D &\rightarrow 0, \\ 
		A &\rightarrow ED\;|\;BB\;|\;B, \\ 
		E &\rightarrow 1\}
	\end{align*}
\end{description}
\section{Eliminate unit rules}
\begin{description}
	\item[Before] \hfill \\ 
	$G=\left(\{	1, 0\},\;\{ S, B, D, A, E\},\;S,\;P\right)$ with
	\begin{align*}
		P=\{	S &\rightarrow BD\;|\;D\;|\;ABD\;|\;AD, \\ 
		B &\rightarrow A, \\ 
		D &\rightarrow 0, \\ 
		A &\rightarrow ED\;|\;BB\;|\;B, \\ 
		E &\rightarrow 1\}
	\end{align*}
	\item[Step 1] remove circles: \\ 
	$G=\left(\{	1, 0\},\;\{ S, A, D, E\},\;S,\;P\right)$ with
	\begin{align*}
		P=\{	S &\rightarrow AAD\;|\;D\;|\;AD, \\ 
		A &\rightarrow ED\;|\;AA, \\ 
		D &\rightarrow 0, \\ 
		E &\rightarrow 1\}
	\end{align*}
	\item[Step 2] number the nonterminals:
	\begin{align*}
		D&: 1\\
		S&: 0
	\end{align*}
	\item[Step 3] remove unit rules beginning by the highest number: \\ 
	$G=\left(\{	0, 1\},\;\{ S, A, D, E\},\;S,\;P\right)$ with
	\begin{align*}
		P=\{	S &\rightarrow AAD\;|\;AD\;|\;0, \\ 
		A &\rightarrow ED\;|\;AA, \\ 
		D &\rightarrow 0, \\ 
		E &\rightarrow 1\}
	\end{align*}
\end{description}
\section{Chomsky - Normal - Form}
\begin{description}
	\item[Before]
	$G=\left(\{	0, 1\},\;\{ S, A, D, E\},\;S,\;P\right)$ with
	\begin{align*}
		P=\{	S &\rightarrow AAD\;|\;AD\;|\;0, \\ 
		A &\rightarrow ED\;|\;AA, \\ 
		D &\rightarrow 0, \\ 
		E &\rightarrow 1\}
	\end{align*}
	\item[Step 1] rules in form of $A \rightarrow a$ are already in chomsky normal form and we keep them.
	\item[Step 2] in all other rules replace every appearance of Terminal a through a new Nonterminal $X_a$ and add the rule $X_a \rightarrow a$.
	$G=\left(\{	0, 1\},\;\{ S, A, D, E\},\;S,\;P\right)$ with
	\begin{align*}
		P=\{	S &\rightarrow AAD\;|\;AD\;|\;0, \\ 
		A &\rightarrow ED\;|\;AA, \\ 
		D &\rightarrow 0, \\ 
		E &\rightarrow 1\}
	\end{align*}
	\item[Step 3] in all rules that contain more than two nonterminals, add a new nonterminal that points to the end of the rule.
	$G=\left(\{	0, 1\},\;\{ S, A, P_1, D, E\},\;S,\;P\right)$ with
	\begin{align*}
		P=\{	S &\rightarrow AP_1\;|\;AD\;|\;0, \\ 
		A &\rightarrow ED\;|\;AA, \\ 
		P_1 &\rightarrow AD, \\ 
		D &\rightarrow 0, \\ 
		E &\rightarrow 1\}
	\end{align*}
\end{description}
\end{document}