\begin{description}
	\item[Before] \hfill \\ 
		$G=(\{	0, 1\},\;\{ S, A, D, E\},\;S,\;R)$ with
	\begin{align*}
		R=\{	S &\rightarrow AD\;|\;0\;|\;AAD, \\ 
		A &\rightarrow ED\;|\;AA, \\ 
		D &\rightarrow 0, \\ 
		E &\rightarrow 1\}
	\end{align*}
	\item[Step 1] \hfill \\ 
	Rules in form A  $\rightarrow$  a are already in chomsky normal form and we keep them.\\ 
		\item[Step 2] \hfill \\ 
	In every other rule replace every appearance of a terminal a through a new nonterminal.\\ 
	$G=(\{	0, 1\},\;\{ S, A, D, E\},\;S,\;R)$ with
	\begin{align*}
		R=\{	S &\rightarrow AD\;|\;0\;|\;AAD, \\ 
		A &\rightarrow ED\;|\;AA, \\ 
		D &\rightarrow 0, \\ 
		E &\rightarrow 1\}
	\end{align*}
	\item[Step 3] \hfill \\ 
	In every rule that contain more than two nonterminals, add a new nonterminal that points to the end of the rule.\\ 
	$G=(\{	0, 1\},\;\{ S, A, P_{0}, D, E\},\;S,\;R)$ with
	\begin{align*}
		R=\{	S &\rightarrow AP_{0} \;|\;AD\;|\;0, \\ 
		A &\rightarrow ED\;|\;AA, \\ 
		P_{0}  &\rightarrow AD, \\ 
		D &\rightarrow 0, \\ 
		E &\rightarrow 1\}
	\end{align*}
\end{description}